theories/cnf.v
@@ -1,0 +1,123 @@
+From mathcomp Require Import ssreflect ssrfun ssrbool eqtype ssrnat seq.
+From resssr Require Import prelude decset model.
+
+Section Cnf.
+
+(** Logic language *)
+Inductive lprop : Type :=
+  | And of lprop & lprop
+  | Or  of lprop & lprop
+  | Neg of lprop
+  | Atom of nat.
+
+Definition Impl (f1 f2 : lprop) : lprop := Or (Neg f1) f2.
+
+Fixpoint eval_lprop (m : val) (f : lprop) : bool :=
+  match f with
+  | And f1 f2 => eval_lprop m f1 && eval_lprop m f2
+  | Or  f1 f2 => eval_lprop m f1 || eval_lprop m f2
+  | Neg f     => ~~ eval_lprop m f
+  | Atom a    => a \in m
+  end.
+
+Inductive precnf : Type :=
+  | AndP of precnf & precnf
+  | OrP  of precnf & precnf
+  | LitP of lit.
+
+(** Conversion algorithm from LProp to PreCnf *)
+Fixpoint remove_neg' (sign : bool) (f : lprop) : precnf :=
+  match f with
+  | And a b =>
+    if sign then AndP (remove_neg' sign a) (remove_neg' sign b)
+    else OrP (remove_neg' false a) (remove_neg' false b)
+  | Or a b =>
+    if sign then OrP (remove_neg' sign a) (remove_neg' sign b)
+    else AndP (remove_neg' false a) (remove_neg' false b)
+  | Neg a =>
+    if sign then remove_neg' false a
+    else remove_neg' true a
+  | Atom n =>
+    if sign then LitP (pos n)
+    else LitP (neg n)
+  end.
+
+Definition remove_neg := remove_neg' true.
+
+Fixpoint eval_precnf (m : val) (f : precnf) : bool :=
+  match f with
+  | AndP f1 f2 => eval_precnf m f1 && eval_precnf m f2
+  | OrP f1 f2 => eval_precnf m f1 || eval_precnf m f2
+  | LitP l => valLit l m
+  end.
+
+  (* [remove_neg' false] inverse the denotations *)
+Lemma remove_neg_false_negb f m :
+  eval_precnf m (remove_neg' false f) = ~~ eval_precnf m (remove_neg' true f).
+Proof.
+elim: f=>[l IHl r IHr|l IHl r IHr|l IH|n] //=.
+- by rewrite negb_and IHl IHr.
+- by rewrite negb_or IHl IHr.
+by rewrite IH negbK.
+Qed.
+
+Theorem remove_neg_correct f m : eval_lprop m f = eval_precnf m (remove_neg f).
+Proof.
+elim: f=>[l IHl r IHr|l IHl r IHr|l IH|n] //=.
+- by rewrite IHl IHr.
+- by rewrite IHl IHr.
+by rewrite IH remove_neg_false_negb.
+Qed.
+
+(** Distribute a clause on a set of clauses *)
+Definition merge_clause (c : clause) (f : form) :=
+  map (cat c) f.
+
+(** Double distribute a set of clauses on another one *)
+Fixpoint merge (f f' : form) : form :=
+  if f is c::f0
+    then merge_clause c f' ++ merge f0 f'
+    else [::].
+
+(** PreCnf to Formula conversion *)
+Fixpoint cnf' (f : precnf) : form :=
+  match f with
+  | AndP a b => cnf' a ++ cnf' b
+  | OrP a b => merge (cnf' a) (cnf' b)
+  | LitP a => [::[::a]]
+  end.
+
+(** CNF conversion *)
+Definition cnf (f : lprop) : form :=
+  cnf' (remove_neg f).
+
+(* [merge_clause] preserve the semantic *)
+Theorem merge_clause_correct c f m :
+  valForm (merge_clause c f) m = valClause c m || valForm f m.
+Proof.
+elim: f=>[|c' f IH]/=; first by rewrite orbT.
+by rewrite valClause_cat IH orb_andr.
+Qed.
+
+(* [merge] preserve the semantic *)
+Theorem merge_correct f f' m :
+  valForm f m || valForm f' m = valForm (merge f f') m.
+Proof.
+elim: f=>//= c f IH.
+by rewrite valForm_cat -IH merge_clause_correct orb_andl.
+Qed.
+
+(* [cnf'] preserve the semantic *)
+Theorem cnf'_correct f m : eval_precnf m f = valForm (cnf' f) m.
+Proof.
+elim: f=>/=[l IHl r IHr|l IHl r IHr|l].
+- by rewrite IHl IHr valForm_cat.
+- by rewrite IHl IHr merge_correct.
+by rewrite andbT orbF.
+Qed.
+
+(* [cnf] preserve the semantic *)
+Theorem cnf_correct f m : eval_lprop m f = valForm (cnf f) m.
+Proof. by rewrite /cnf remove_neg_correct cnf'_correct. Qed.
+
+End Cnf.
